theories/Prelude/PreludeUtil.v
@@ -1069,23 +1069,30 @@ Module MyUtil.
 
 (** "resolver" *)
 
-  Global Hint Rewrite @in_app_iff : khan_hints.
-  Global Hint Rewrite @in_remove_iff : khan_hints.
-  Global Hint Rewrite @in_map_iff : khan_hints.
-  Global Hint Rewrite @forallb_app : khan_hints.
-  Global Hint Rewrite @forallb_true_iff : khan_hints.
-  Global Hint Rewrite @andb_true_iff : khan_hints.
-  Global Hint Rewrite @orb_true_iff : khan_hints.
-  Global Hint Rewrite @negb_true_iff : khan_hints.
-  Global Hint Rewrite @andb_false_iff : khan_hints.
-  Global Hint Rewrite @orb_false_iff : khan_hints.
-  Global Hint Rewrite @negb_false_iff : khan_hints.
-  Global Hint Rewrite @Nat.eqb_eq : khan_hints.
-  Global Hint Rewrite @Nat.eqb_neq : khan_hints.
-  Global Hint Rewrite @not_true_iff_false : khan_hints.
-  Global Hint Rewrite @not_false_iff_true : khan_hints.
+  Ltac resolver1 :=
+    simpl in *;
+    first
+    [ rewrite in_app_iff in *
+    | rewrite in_remove_iff in *
+    | rewrite orb_false_iff in *
+    | rewrite forallb_app in *
+    | rewrite andb_true_iff in *
+    | rewrite orb_true_iff in *
+    | rewrite negb_true_iff in *
+    | rewrite andb_false_iff in *
+    | rewrite negb_false_iff in *
+    | rewrite Nat.eqb_eq in *
+    | rewrite Nat.eqb_neq in *
+    | rewrite forallb_true_iff in *
+    | rewrite in_map_iff in *
+    | rewrite not_true_iff_false in *
+    | rewrite not_false_iff_true in *
+    ]
+  .
 
-  Ltac resolver := ii; simpl in *; autorewrite with khan_hints using eauto; try now (subst; firstorder).
+  Ltac resolver :=
+    repeat resolver1; repeat (try intro; try resolver1; try now (subst; firstorder))
+  .
 
 End MyUtil.
 
